src/Avl_tree.v
@@ -1,0 +1,787 @@
+Require Import Core.
+Require Import Coq.Lists.List.
+Import ListNotations.
+Import Equal.Notations.
+       
+Set Implicit Arguments.
+
+Module Make (S:SORTABLE).
+  Import Relation.
+
+(** * Sortable *)
+(*    ======== *)
+  Section sortable.
+    Definition A:Set :=  S.T.
+
+    Theorem transitive: Transitive S.Less_equal.
+    Proof
+      match S.is_linear_preorder with
+        conj _ tr => tr
+      end.
+
+    Theorem reflexive: Reflexive S.Less_equal.
+    Proof
+      match S.is_linear_preorder with
+        conj d _ =>
+        dichotomic_is_reflexive d
+      end.
+
+  End sortable.
+  Notation "a <= b"  := (S.Less_equal a b) (at level 70).
+  Notation "a <=? b" := (S.is_less_equal a b) (at level 70).
+  Notation "( 'transitivity_chain:' x , y , .. , z )" :=
+    (transitive .. (transitive x y) .. z) (at level 0).
+    
+
+  Definition Equivalent (a b:A): Prop := a <= b /\ b <= a.
+
+
+
+(** * List *)
+(*    ==== *)
+  Module List.
+    Definition L: Set := list A.
+
+    Inductive Permutation: L -> L -> Prop :=
+    | perm_empty:
+        Permutation [] []
+    | perm_prefix:
+        forall x a b, Permutation a b -> Permutation (x::a) (x::b)
+    | perm_swap:
+        forall x y a,  Permutation (x::y::a) (y::x::a)
+    | perm_transitive:
+        forall a b c,  Permutation a b -> Permutation b c -> Permutation a c.
+  End List.
+
+
+
+(** * Basic Definitions *)
+(*    ================= *)
+  Section basic_definitions.
+    Inductive Balance: Set :=
+      balanced: Balance
+    | left_leaning: Balance.
+
+    Inductive T :=
+      empty: T
+    | node:  Balance -> A -> T -> T -> T.
+
+    Fixpoint height (t:T): nat :=
+      match t with
+      | empty => 0
+      | node _ _ t1 t2 => 1 + max (height t1) (height t2)
+      end.
+
+    Definition Node (t:T): Prop :=
+      match t with
+      | empty => False
+      | node _ _ _ _ => True
+      end.
+
+    Inductive Domain: T -> A -> Prop :=
+    | domain_node:
+        forall x b a t1 t2,
+          x = a -> Domain (node b a t1 t2) x
+    | domain_left:
+        forall x a b t1 t2,
+          Domain t1 x -> Domain (node b a t1 t2) x
+    | domain_right:
+        forall x a b t1 t2,
+          Domain t2 x -> Domain (node b a t1 t2) x.
+
+
+    Theorem node_not_empty:
+      forall (b:Balance) (a:A) (t1 t2: T),
+        node b a t1 t2 <> empty.
+    Proof
+      fun b a t1 t2 p =>
+        Equal.rewrite p Node I.
+
+    Definition is_node (t:T): {Node t} + {~ Node t} :=
+      match t return {Node t} + {~ Node t} with
+        empty => right (fun p:False => match p with end)
+      | node b a t1 t2 => left I
+      end.
+
+    Definition element (t:T): Node t -> A :=
+      match t return Node t -> A with
+      | empty => fun p:Node empty => match p with end
+      | node _ a _ _ => fun _ => a
+      end.
+
+    Definition left_son (t:T): Node t -> T :=
+      match t return Node t -> T with
+      | empty => fun p:Node empty => match p with end
+      | node _ _ t1 _ => fun _ => t1
+      end.
+
+    Definition right_son (t:T): Node t -> T :=
+      match t return Node t -> T with
+      | empty => fun p:Node empty => match p with end
+      | node _ _ _ t2 => fun _ => t2
+      end.
+
+
+    Definition balance (t:T): Balance :=
+      match t with
+      | empty => balanced
+      | node b _ _ _ => b
+      end.
+
+    Fixpoint least (t:T): Node t -> A :=
+      match t return Node t -> A with
+      | empty =>
+        fun p => match p with end
+      | node b a t1 t2 =>
+        match is_node t1 with
+          left  pt1 => fun _ => least t1 pt1
+        | right pt1 => fun _ => a
+        end
+      end.
+
+    Fixpoint greatest (t:T): Node t -> A :=
+      match t return Node t -> A with
+      | empty =>
+        fun p => match p with end
+      | node b a t1 t2 =>
+        match is_node t2 with
+          left  pt2 => fun _ => greatest t2 pt2
+        | right pt2 => fun _ => a
+        end
+      end.
+  End basic_definitions.
+
+
+(** * Module 'Node' Describing the Content of a Node *)
+(*    ============================================== *)
+  Module Node.
+    Import Equal.Notations.
+    Record N := make { balance:Balance; element:A; left:T; right:T}.
+
+    Print balance.
+    Print N.
+    Definition Tree_node (n:N) (t:T): Prop :=
+      t = node n.(balance) n.(element) n.(left) n.(right).
+
+    Definition tree_node (t:T): Node t -> {n:N | Tree_node n t} :=
+      match t return Node t -> {n | Tree_node n t} with
+      | empty =>
+        fun p => match p with end
+      | node b a t1 t2 =>
+        fun _ =>
+          let n := make b a t1 t2 in
+          let p: Tree_node n (node b a t1 t2) :=
+              (equal_arguments: eq_refl, eq_refl, eq_refl, eq_refl)
+          in
+          exist _ n p
+      end.
+  End Node.
+
+
+(** * Balanced Trees *)
+(*    ============== *)
+  Section balanced.
+    Inductive Balanced: nat -> Balance -> T -> Prop :=
+      balanced_empty:
+        Balanced 0 balanced empty
+    | balanced_perfect:
+        forall h b1 t1 b2 t2 h_new a,
+          h_new = 1 + h ->
+          Balanced h b1 t1 ->
+          Balanced h b2 t2 ->
+          Balanced h_new balanced (node balanced a t1 t2)
+    | balanced_left_leaning:
+        forall h1 b1 t1 h2 b2 t2 h_new a,
+          h1 = 1 + h2 ->
+          h_new = 2 + h2 ->
+          Balanced h1 b1 t1 ->
+          Balanced h2 b2 t2 ->
+          Balanced h_new left_leaning (node left_leaning a t1 t2).
+
+    Definition Balanced_tree (t:T): Prop :=
+      Balanced (height t) (balance t) t.
+
+
+    Inductive Balanced2: nat -> T -> Prop :=
+    | bal_empty: Balanced2 0 empty
+    | bal_equal: forall h t1 t2 a,
+        Balanced2 h t1 ->
+        Balanced2 h t2 ->
+        Balanced2 (1+h) (node balanced a t1 t2)
+    | bal_left: forall h t1 t2 a,
+        Balanced2 (1+h) t1 ->
+        Balanced2 h t2 ->
+        Balanced2 (2+h) (node left_leaning a t1 t2).
+
+
+    Theorem height_consistent2:
+      forall (h:nat) (t:T), Balanced2 h t -> h = height t.
+    Proof
+      fix f h t p {struct p}: h = height t :=
+      (* height (node _ _ t1 t2) = 1 + max (height t1) (height t2)
+       *)
+      match p in Balanced2 h t return h = height t with
+      | bal_empty =>
+        eq_refl
+      | @bal_equal h t1 t2 a bal1 bal2 =>
+        (equality_chain:
+           (eq_refl: 1 + h = _)
+           ,
+           (let p : max h h = h := max_l h h (le_n h) in
+            Equal.inject (Equal.flip p) (fun x => 1 + x)
+            : _ = 1 + max h h)
+           ,
+           (let ht1: h = height t1 := f h t1 bal1 in
+            Equal.inject ht1 (fun x => 1 + max x h)
+            : _ = 1 + max (height t1) h)
+           ,
+           (let ht2: h = height t2 := f h t2 bal2 in
+            Equal.inject ht2 (fun x => 1 + max (height t1) x)
+            : _ = 1 + max (height t1) (height t2))
+           ,
+           (eq_refl: _ = height (node balanced a t1 t2))
+        )
+      | @bal_left h t1 t2 a bal1 bal2 =>
+        (equality_chain:
+           (eq_refl: 2 + h = _)
+           ,
+           (let p: max (1+h) h = 1 + h := max_l (1+h) h (le_S _ h (le_n h)) in
+            Equal.inject (Equal.flip p) (fun x => 1 + x)
+            : _ = 1 + max (1+h) h)
+           ,
+           (let ht1: 1 + h = height t1 := f (1+h) t1 bal1 in
+            Equal.inject ht1 (fun x => 1 + max x h)
+            : _ = 1 + max (height t1) h)
+           ,
+           (let ht2: h = height t2 := f h t2 bal2 in
+            Equal.inject ht2 (fun x => 1 + max (height t1) x)
+            : _ = 1 + max (height t1) (height t2))
+           ,
+           (eq_refl: _ = height (node left_leaning a t1 t2))
+        )
+      end.
+
+
+    Theorem height_consistent:
+      forall (h:nat) (b:Balance) (t:T), Balanced h b t -> h = height t.
+    Proof.
+      refine(
+      fix f h b t p {struct p}: h = height t  :=
+        match p in Balanced h b t return h = height t with
+        | balanced_empty => eq_refl
+        | @balanced_perfect h b1 t1 b2 t2 h_new a ph p1 p2 =>
+          let pht1: h = height t1 := f h b1 t1 p1 in
+          let pht2: h = height t2 := f h b2 t2 p2 in
+          _
+        | @balanced_left_leaning h1 b1 t1 h2 b2 t2 h_new a ph1 ph_new p1 p2 =>
+          let pht1: h1 = height t1 := f h1 b1 t1 p1 in
+          let pht2: h2 = height t2 := f h2 b2 t2 p2 in
+          _
+        end).
+      - simpl. rewrite <- pht1. rewrite <- pht2.
+        rewrite max_l. assumption. apply le_n.
+      - simpl. rewrite <- pht1. rewrite <- pht2.
+        Search (max _ _).
+        rewrite max_l. rewrite ph_new. rewrite ph1. reflexivity.
+        rewrite ph1. apply le_S. apply le_n.
+    Qed.
+
+    Theorem balanced_is_balanced_tree:
+      forall (h:nat) (b:Balance) (t:T),
+        Balanced h b t ->
+        Balanced_tree t.
+    Proof.
+      refine (
+          fix f h b t pbal :=
+            match pbal in Balanced h b t return Balanced_tree t with
+            | balanced_empty =>
+              balanced_empty
+            | @balanced_perfect
+                h b1 t1 b2 t2 h_new a
+                ph pbal1 pbal2 =>
+              let ph1: h = height t1 := @height_consistent h b1 t1 pbal1 in
+              let ph2: h = height t2 := @height_consistent h b2 t2 pbal2 in
+              _
+            | @balanced_left_leaning
+                h1 b1 t1 h b2 t2 h_new a
+                ph1 phnew pbal1 pbal2 =>
+              let pht1: h1 = height t1 := @height_consistent h1 b1 t1 pbal1 in
+              let pht2: h  = height t2 := @height_consistent h  b2 t2 pbal2 in
+              _
+            end).
+      - unfold Balanced_tree. simpl. rewrite <- ph1. rewrite <- ph2. rewrite max_l.
+        apply balanced_perfect with (h:=h)(b1:=b1)(b2:=b2).
+        reflexivity. assumption. assumption. apply le_n.
+      - unfold Balanced_tree.  simpl. rewrite <- pht1. rewrite <- pht2.
+        rewrite max_l.
+        apply balanced_left_leaning with (h1:=h1) (b1:=b1) (h2:=h) (b2:=b2).
+        assumption. rewrite ph1. reflexivity. assumption. assumption.
+        rewrite ph1. apply le_S. apply le_n.
+    Qed.
+
+    Theorem balanced_subtree:
+      forall (b:Balance) (h:nat) (t:T),
+        Balanced h b t ->
+        forall p:Node t,
+          Balanced_tree (left_son t p) /\
+          Balanced_tree (right_son t p).
+    Proof
+      fun b h t pbal =>
+        match pbal in Balanced h b t
+              return
+              forall p:Node t,
+                Balanced_tree (left_son t p) /\
+                Balanced_tree (right_son t p)
+        with
+        | balanced_empty =>
+          fun pnode => match pnode with end
+        | @balanced_perfect h b1 t1 b2 t2 h_new a ph pbal1 pbal2 =>
+          fun pnode =>
+            let lson := left_son  (node balanced a t1 t2) pnode in
+            let rson := right_son (node balanced a t1 t2) pnode in
+            let peq1 : t1 = lson := eq_refl in
+            let peq2 : t2 = rson := eq_refl in
+            let pbal_left: Balanced h b1 lson :=
+                Equal.rewrite peq1 (Balanced h b1) pbal1 in
+            let pbal_right: Balanced h b2 rson :=
+                Equal.rewrite peq2 (Balanced h b2) pbal2 in
+            conj
+              (@balanced_is_balanced_tree h b1 lson pbal_left)
+              (@balanced_is_balanced_tree h b2 rson pbal_right)
+        | @balanced_left_leaning h1 b1 t1 h b2 t2 h_new a ph1 phnew pbal1 pbal2 =>
+          fun pnode =>
+            let lson := left_son  (node left_leaning a t1 t2) pnode in
+            let rson := right_son (node left_leaning a t1 t2) pnode in
+            let peq1 : t1 = lson := eq_refl in
+            let peq2 : t2 = rson := eq_refl in
+            let pbal_left: Balanced h1 b1 lson :=
+                Equal.rewrite peq1 (Balanced h1 b1) pbal1 in
+            let pbal_right: Balanced h b2 rson :=
+                Equal.rewrite peq2 (Balanced h b2) pbal2 in
+            conj
+              (@balanced_is_balanced_tree h1 b1 lson pbal_left)
+              (@balanced_is_balanced_tree h  b2 rson pbal_right)
+        end.
+  End balanced.
+
+
+
+(** * Sorted Trees *)
+(*    ============ *)
+  Section sorted.
+    Inductive Sorted: A -> A -> T -> Prop :=
+      empty_sorted:
+        forall lo hi, lo <= hi -> Sorted lo hi empty
+    | node_sorted:
+        forall lo1 hi1 t1 lo2 hi2 t2 b a,
+          Sorted lo1 hi1 t1 ->
+          Sorted lo2 hi2 t2 ->
+          hi1 <= a ->
+          a <= lo2 ->
+          Sorted lo1 hi2 (node b a t1 t2).
+
+    Theorem guards_consistent:
+      forall (lo hi:A) (t:T),
+        Sorted lo hi t -> lo <= hi.
+    Proof
+      fix f lo hi t s :=
+      match s in Sorted lo hi t return lo <= hi with
+      | @empty_sorted lo hi p => p
+      | @node_sorted lo1 hi1 t1 lo2 hi2 t2 b a s1 s2 le1 le2 =>
+        let p1: lo1 <= hi1 := f lo1 hi1 t1 s1 in
+        let p2: lo2 <= hi2 := f lo2 hi2 t2 s2 in
+        (transitivity_chain: p1, le1, le2, p2)
+      end.
+    
+    Definition Sorted_tree (t:T): Prop :=
+      match is_node t with
+      | left  p => (* p: Node t *)
+        Sorted (least t p) (greatest t p) t
+      | right p => (* p: ~ Node t *)
+        True
+      end.
+
+    Definition Sorted_tree2 (t:T): Prop :=
+      exists lo hi, Sorted lo hi t.
+    
+    Theorem least_consistent:
+      forall (lo hi:A) (t:T),
+        Sorted lo hi t -> forall nd:Node t, lo <= least t nd.
+    Proof
+      let Cond lo t := forall nd:Node t, lo <= least t nd
+      in
+      fix f lo hi t sorted :=
+      match sorted in Sorted lo hi t
+            return Cond lo t
+      with
+      | empty_sorted _ =>
+        fun nd =>
+          match nd with end
+      | @node_sorted lo1 hi1 t1
+                     lo2 hi2 t2
+                     b a
+                     s1 s2 le_l_a le_a_r =>
+        fun nd =>
+          (match
+              t1
+              return (Cond lo1 t1) -> lo1 <= least (node b a t1 t2) nd
+           with
+           | empty =>
+             fun _ =>
+               Equal.rewrite
+                 (eq_refl : a = least (node b a empty t2) nd)
+                 (fun x => lo1 <= x)
+                 (* lo1 <= hi1 <= a *)
+                 (transitivity_chain: guards_consistent s1, le_l_a)
+           | node b1 a1 t11 t12 =>
+             let t := node b1 a1 t11 t12 in
+             fun p1: forall nd1,
+                 lo1 <= least t nd1 =>
+               Equal.rewrite
+                 (eq_refl (least t I))
+                 (fun x => lo1 <= least t I)
+                 (p1 I)
+           end) (f lo1 hi1 t1 s1)
+      end.
+
+
+    Theorem greatest_consistent:
+      forall (lo hi:A) (t:T),
+        Sorted lo hi t -> forall nd:Node t, greatest t nd <= hi.
+    Proof
+      let Cond hi t := forall nd:Node t, greatest t nd <= hi
+      in
+      fix f lo hi t sorted :=
+      match sorted in Sorted lo hi t
+            return Cond hi t
+      with
+      | empty_sorted _ =>
+        fun nd =>
+          match nd with end
+      | @node_sorted lo1 hi1 t1
+                     lo2 hi2 t2
+                     b a
+                     s1 s2 le_l_a le_a_r =>
+        fun nd =>
+          (match
+              t2
+              return (Cond hi2 t2) -> greatest (node b a t1 t2) nd <= hi2
+           with
+           | empty =>
+             fun _ =>
+               Equal.rewrite
+                 (eq_refl : a = greatest (node b a t1 empty) nd)
+                 (fun x => x <= hi2)
+                 (* a <= lo2 <= hi2 *)
+                 (transitivity_chain: le_a_r, guards_consistent s2)
+           | node b2 a2 t21 t22 =>
+             let t := node b2 a2 t21 t22 in
+             fun p1: forall nd2,
+                 greatest t nd2 <= hi2 =>
+               Equal.rewrite
+                 (eq_refl (greatest t I))
+                 (fun x => greatest t I <= hi2)
+                 (p1 I)
+           end) (f lo2 hi2 t2 s2)
+      end.
+
+    Theorem root_element_sorted:
+      forall (t:T) (lo hi:A),
+        Sorted lo hi t ->
+        forall (nd:Node t),
+          lo <= element t nd /\ element t nd <= hi.
+    Proof
+      (* match sorted:
+         a) empty: by contradiction
+         b) node:  lo1 <= hi1  (guards_consistent)
+                   hi1 <= a    (Sorted ...)
+                   a = element t nd
+                   a <= lo2    (Sorted ...)
+                   lo2 <= hi2  (guards_consistent)
+       *)
+      let Cond lo hi t nd :=
+          lo <= element t nd /\ element t nd <= hi
+      in
+      fun t lo hi sorted =>
+        match sorted in Sorted lo hi t
+              return forall nd, Cond lo hi t nd
+        with
+        | empty_sorted _ =>
+          fun nd =>
+            match nd with end
+        | @node_sorted lo1 hi1 t1
+                       lo2 hi2 t2
+                       b a
+                       s1 s2 le_hi1_a le_a_lo2 =>
+          (* goal: forall nd: Node (node b a t1 t2),
+                      lo1 <= element (node b a t1 t2) nd *)
+          fun nd =>
+            let eq_a: a = element (node b a t1 t2) nd := eq_refl in
+            conj
+              (Equal.rewrite
+                 eq_a
+                 (fun x => lo1 <= x)
+                 (transitivity_chain: guards_consistent s1,le_hi1_a))
+              (Equal.rewrite
+                 eq_a
+                 (fun x => x <= hi2)
+                 (transitivity_chain: le_a_lo2, guards_consistent s2))
+        end.
+
+
+    Theorem least_greatest_consistent:
+      forall (lo hi:A) (t:T),
+        Sorted lo hi t ->
+        forall nd:Node t, Sorted (least t nd) (greatest t nd) t.
+    Proof
+      let Cond t nd: Prop := Sorted (least t nd) (greatest t nd) t
+      in
+      fun lo hi t sorted =>
+        match sorted in Sorted lo hi t
+              return forall nd, Cond t nd
+        with
+        | empty_sorted _ =>
+          fun nd =>
+            match nd with end
+        | @node_sorted lo1 hi1 t1
+                       lo2 hi2 t2
+                       b a
+                       s1 s2 le_hi1_a le_a_lo2 =>
+          _
+        end.
+    Print ex.
+
+    Theorem sorted_is_sorted:
+      forall (t:T),
+        Sorted_tree2 t ->
+        forall  (nd:Node t),
+          Sorted (least t nd) (greatest t nd) t.
+    Proof
+      let Cond t nd := Sorted (least t nd) (greatest t nd) t
+      in
+      fun t exist_lo_hi =>
+        match exist_lo_hi with
+        | ex_intro _ lo exist_hi =>
+          match exist_hi with
+            ex_intro _ hi sorted =>
+            match sorted in Sorted lo hi t
+                  return forall nd, Cond t nd
+            with
+            | empty_sorted _ =>
+              fun nd => match nd with end
+            | @node_sorted lo1 hi1 t1
+                           lo2 hi2 t2
+                           b a
+                           s1 s2 le_hi1_a le_a_lo2 =>
+              fun nd =>
+                let t_ := node b a t1 t2 in
+                (* goal: Sorted (least t_ nd) (greatest t_ nd) t_
+                 *)
+                _
+            end           
+          end
+        end.
+  End sorted.
+
+    
+  Section blabla.
+    Inductive Permutation: T -> T -> Prop :=
+    | perm_empty:
+        Permutation empty empty
+    | perm_left:
+        forall b1 b2 a1 a2 t1 t2 t3,
+          Permutation
+            (node b1 a1 (node b2 a2 t1 t2) t3)
+            (node b1 a2 (node b2 a1 t1 t2) t3)
+    | perm_right:
+        forall b1 b2 a1 a2 t1 t2 t3,
+          Permutation
+            (node b1 a1 t1 (node b2 a2 t2 t3))
+            (node b1 a2 t1 (node b2 a1 t2 t3))
+    | perm_root:
+        forall t u v w a b,
+          Permutation t u ->
+          Permutation v w ->
+          Permutation (node b a t v) (node b a u w)
+    | perm_transitive:
+        forall t1 t2 t3,
+          Permutation t1 t2 -> Permutation t2 t3 -> Permutation t1 t3.
+
+
+    (* Replace a t1 t2: An element of 't1' equivalent to 'a' has been replaced
+                        by 'a' resulting in 't2'. *)
+    Inductive Replaced: A -> T -> T -> Prop :=
+    | replaced_root:
+        forall x a b t1 t2,
+          Equivalent x a ->
+          Replaced x (node b a t1 t2) (node b x t1 t2)
+    | replaced_left:
+        forall x t1 t2 b a t,
+          Replaced x t1 t2 ->
+          Replaced x (node b a t1 t) (node b a t2 t)
+    | replaced_right:
+        forall x t1 t2 b a t,
+          Replaced x t1 t2 ->
+          Replaced x (node b a t t1) (node b a t t2)
+    .
+
+    Definition Avl (t:T): Prop :=
+      match is_node t with
+      | left  p => Balanced (height t) (balance t) t
+                   /\
+                   Sorted (least t p) (greatest t p) t
+      | right _ => True
+      end.
+
+    Fixpoint inorder (t:T): List.L :=
+      match t with
+        empty => []
+      | node b a t1 t2 => inorder t1 ++ a :: inorder t2
+      end.
+
+  End blabla.
+
+  Theorem avl_subtree:
+    forall (a:A) (b:Balance) (t1 t2:T),
+      Avl (node b a t1 t2) -> Avl t1 /\ Avl t2.
+  Proof.
+    intros a b t1 t2 pavl. unfold Avl in pavl. unfold is_node in pavl.
+    destruct pavl as [pbal psorted].
+    split.
+    - unfold Avl.
+    -
+    fun a b t1 t2 pavl =>
+      match pavl with
+        left p => _
+                    right
+
+      _.
+
+  Definition add_root (a:A) (t:T): T :=
+    node left_leaning a t empty.
+
+
+  Definition Inserted (x:A) (t u:T): Prop :=
+    List.Permutation (x :: inorder t) (inorder u).
+
+  Definition Avl_inserted (x:A) (t u:T): Prop :=
+    Avl u /\ Inserted x t u.
+  Check Inserted.
+
+
+  Theorem insert_empty:
+    forall x:A,
+      Avl_inserted x empty (node balanced x empty empty).
+  Proof.
+    intro x. split.
+    - unfold Avl. unfold is_node. split.
+      -- simpl. eapply balanced_perfect; apply balanced_empty.
+      -- simpl. apply node_sorted with (hi1:=x) (lo2:=x);
+                  repeat (apply empty_sorted); repeat (apply reflexive).
+    - unfold Inserted. simpl. apply List.perm_prefix. apply List.perm_empty.
+  Qed.
+
+  Section insertion.
+    Definition insert:
+      forall (a:A) (t:T),
+        Avl t ->
+        Either.T {u:T | Avl_inserted a t u} {u:T | Replaced a t u}
+      :=
+      fix f x t :=
+        match t
+              return Avl t -> Either.T {u| Avl_inserted x t u} {u| Replaced x t u}
+        with
+        | empty =>
+          fun _ =>
+            let u := node balanced x empty empty in
+            Either.left _ (exist _ u (insert_empty x))
+        | node bal a t1 t2 =>
+          fun pavl_t =>
+            match x <=? a, a <=? x with
+            | left p1, left p2  =>
+              (* x and a are equivalent, replace *)
+              let u := node bal x t1 t2 in
+              let p_replace: Replaced x (node bal a t1 t2) u :=
+                  @replaced_root x a bal t1 t2 (conj p1 p2)
+              in
+              Either.right _ (exist _ u p_replace)
+            | left p1, _  =>
+              (* insert into left subtree *)
+              let pavl_t1: Avl t1 := _ in
+              match f x t1 pavl_t1 with
+              | Either.left _ sig_ins_t1 =>
+                _
+              | Either.right _ sig_repl_t1 =>
+                _
+              end
+            | right p1, _  =>
+              (* insert into right subtree *)
+              _
+            end
+        end.
+  End insertion.
+
+
+
+  Section draft.
+    Inductive Avl2: A -> A -> nat -> Balance -> T -> Prop :=
+      avl_empty:
+        forall lo hi, lo <= hi -> Avl2 lo hi 0 balanced empty
+    | avl_balanced:
+        forall lo1 hi1 b1 t1 lo2 hi2 b2 t2 h a,
+          Avl2 lo1 hi1 h b1 t1 ->
+          Avl2 lo2 hi2 h b2 t2 ->
+          hi1 <= a ->
+          a <= lo2 ->
+          Avl2 lo1 hi2 (1+h) balanced (node balanced a t1 t2)
+    | avl_left_leaning:
+        forall lo1 hi1 b1 t1 lo2 hi2 b2 t2 h a,
+          Avl2 lo1 hi1 (1+h) b1 t1 ->
+          Avl2 lo2 hi2 h b2 t2 ->
+          hi1 <= a ->
+          a <= lo2 ->
+          Avl2 lo1 hi2 (2+h) left_leaning (node left_leaning a t1 t2).
+
+    Theorem extend_guards:
+      forall (lo_new lo hi hi_new:A) (h:nat) (b:Balance) (t:T),
+        Avl2 lo hi h b t ->
+        lo_new <= lo ->
+        hi <= hi_new ->
+        Avl2 lo_new hi_new h b t.
+    Proof
+      fix f lo_new lo hi hi_new h b t p_avl:=
+      match
+          p_avl in Avl2 lo hi h b t
+          return lo_new <= lo -> hi <= hi_new -> Avl2 lo_new hi_new h b t
+      with
+        @avl_empty lo hi p => (* p: lo <= hi *)
+        fun (p1:lo_new<=lo) (p2:hi<=hi_new) =>
+          let pguard: lo_new <= hi_new :=
+              transitive (transitive p1 p) p2
+          in
+          @avl_empty lo_new hi_new pguard
+      | @avl_balanced
+          lo1 hi1 b1 t1
+          lo2 hi2 b2 t2 h a
+          p_avl_t1 p_avl_t2 pleft pright =>
+        fun (p1:lo_new<=lo1) (p2:hi2<=hi_new) =>
+          let p_avl_t1_new :=
+              f lo_new lo1 hi1 hi1 h b1 t1 p_avl_t1 p1 (reflexive hi1) in
+          let p_avl_t2_new :=
+              f lo2 lo2 hi2 hi_new h b2 t2 p_avl_t2 (reflexive lo2) p2 in
+          avl_balanced p_avl_t1_new p_avl_t2_new pleft pright
+      | @avl_left_leaning
+          lo1 hi1 b1 t1
+          lo2 hi2 b2 t2
+          h a
+          p_avl_t1 p_avl_t2 pleft pright =>
+        fun (p1:lo_new<=lo1) (p2:hi2<=hi_new) =>
+          let p_avl_t1_new :=
+              f lo_new lo1 hi1 hi1 (1+h) b1 t1 p_avl_t1 p1 (reflexive hi1) in
+          let p_avl_t2_new :=
+              f lo2 lo2 hi2 hi_new h b2 t2 p_avl_t2 (reflexive lo2) p2 in
+          avl_left_leaning p_avl_t1_new p_avl_t2_new pleft pright
+      end
+    .
+  End draft.
+End Make.
